\begin{aibox}{\function}
;; SAT-p

SYNTAX: SAT-p (kb)
\end{aibox}

\begin{aibox}{\examples}
\begin{alltt}
(SAT-p '((<=> A (¬ H)) (<=> P (^ A H)) (<=> H P))) ; T

(SAT-p '((=> (^ P I) L) (=> (¬ P) (¬ L)) (¬ P) L)) ; NIL
\end{alltt}

\end{aibox}

\begin{aibox}{\comments}

\end{aibox}
\begin{aibox}{\answers}

\end{aibox}
\begin{aibox}{\othercomments}

\end{aibox}
\begin{aibox}{\pseudocode}

\end{aibox}
\begin{aibox}{\code}

\begin{alltt}

(defun SAT-p (kb)
  (not (null (encuentra-modelos kb))))

\end{alltt}
\end{aibox}
